make everything except stlcexercises compile, and mirror examples from report

project/Examples.v
@@ -35,10 +35,10 @@ Notation odd := "odd".
 Notation eo := "eo".
 
 Definition fact :=
-t_fix
-  (t_abs f (TArrow TNat TNat)
-    (t_abs "x" TNat
-      (t_if
+  t_fix
+    (t_abs f (TArrow TNat TNat)
+      (t_abs "x" TNat
+        (t_if
           (t_nat_eq (t_nat 0) (t_var "x"))
           (t_nat 1)
           (t_mult
@@ -46,19 +46,19 @@ t_fix
             (t_app (t_var f) (t_pred (t_var "x"))))))).
 
 Example fact_test:
-(t_app fact (t_nat 4)) ==>* (t_nat 24).
+  (t_app fact (t_nat 4)) ==>* (t_nat 24).
 Proof. unfold fact. normalize. Qed.
 
 Definition Either a b :=
   TSCons "Left" a (TSCons "Right" b TSNil).
 
 Example either_test:
-t_match 
-  (t_sum "Right" t_true (Either TNat TBool)) 
-  (t_case_cons "Left" 
-    (t_abs "x"  TNat (t_var "x")) 
-    (t_case_one "Right" (t_abs "x" TBool (t_nat 0))))
-      ==>* t_nat 0.
+  t_match 
+    (t_sum "Right" t_true (Either TNat TBool)) 
+    (t_case_cons "Left" 
+      (t_abs "x"  TNat (t_var "x")) 
+      (t_case_one "Right" (t_abs "x" TBool (t_nat 0))))
+        ==>* t_nat 0.
 Proof.
   eapply multi_step.
   - apply ST_MatchSumTail; easy.
@@ -73,12 +73,20 @@ Definition product :=
       (t_abs "x" (TList TNat)
         (t_match (t_var "x") 
           (t_case_cons "cons"
-            (t_abs "l" (TRCons "head" TNat (TRCons "tail" (TList TNat) TRNil))
-              (t_mult (t_proj (t_var "l") "head") (t_app (t_var "f") (t_proj (t_var "l") "tail"))))
+            (t_abs "l" 
+              (TRCons "head" TNat 
+              	(TRCons "tail" (TList TNat) TRNil))
+              (t_mult 
+              	(t_proj (t_var "l") "head") 
+                (t_app 
+                  (t_var "f") 
+                  (t_proj (t_var "l") "tail"))))
           (t_case_one "nil" (t_abs "_" TRNil (t_nat 1))))))).
 
 Example list_test :
-  t_app product (t_lcons (t_nat 3) (t_lcons (t_nat 7) (t_lnil TNat))) ==>* t_nat 21.
+  t_app product (t_lcons (t_nat 3) 
+    (t_lcons (t_nat 7) (t_lnil TNat))) 
+      ==>* t_nat 21.
 Proof.
   unfold product.
   eapply multi_step. auto.
